AVM/Class/Member.lean
@@ -4,20 +4,20 @@ namespace AVM.Class
 
 structure Constructor {lab : Ecosystem.Label} (cid : lab.ClassId) (constrId : cid.label.ConstructorId) : Type 1 where
   /-- Constructor call body. -/
-  body : constrId.Args.type → Program.{0} lab (ObjectData cid)
+  body : constrId.Args.type → Program.{0} lab.toScope (ObjectData cid)
   /-- Extra constructor logic. The constructor invariant is combined with
       auto-generated constructor body constraints to create the constructor logic. -/
   invariant : (args : constrId.Args.type) → constrId.Signatures args →  Bool
 
 structure Destructor {lab : Ecosystem.Label} (cid : lab.ClassId) (destructorId : cid.label.DestructorId) : Type 1 where
   /-- Destructor call body. -/
-  body : (self : Object cid) → destructorId.Args.type → Program.{0} lab PUnit
+  body : (self : Object cid) → destructorId.Args.type → Program.{0} lab.toScope PUnit
   /-- Extra destructor logic. -/
   invariant : (self : Object cid) → (args : destructorId.Args.type) → destructorId.Signatures args → Bool
 
 structure Method {lab : Ecosystem.Label} (cid : lab.ClassId) (methodId : cid.label.MethodId) : Type 1 where
   /-- Method call body. -/
-  body : (self : Object cid) → methodId.Args.type → Program lab (Object cid)
+  body : (self : Object cid) → methodId.Args.type → Program lab.toScope (Object cid)
   /-- Extra method logic. The method invariant is combined with auto-generated
       method body constraints to create the method logic. -/
   invariant : (self : Object cid) → (args : methodId.Args.type) → methodId.Signatures args → Bool
